@prefix : <http://lenticularlens.org/voidPlus#> .
@prefix cc: <https://creativecommons.org/ns#> .
@prefix owl: <http://www.w3.org/2002/07/owl#> .
@prefix rdf: <http://www.w3.org/1999/02/22-rdf-syntax-ns#> .
@prefix xml: <http://www.w3.org/XML/1998/namespace> .
@prefix xsd: <http://www.w3.org/2001/XMLSchema#> .
@prefix rdfs: <http://www.w3.org/2000/01/rdf-schema#> .
@prefix void: <http://rdfs.org/ns/void#> .
@prefix dcterms: <http://purl.org/dc/terms/> .
@prefix voidPlus: <http://lenticularlens.org/voidPlus/> .
@base <http://lenticularlens.org/voidPlus> .

<http://lenticularlens.org/voidPlus> rdf:type owl:Ontology .

#################################################################
#    Object Properties
#################################################################

###  http://lenticularlens.org/voidPlus/hasAlgorithm
voidPlus:hasAlgorithm rdf:type owl:ObjectProperty ,
                               owl:FunctionalProperty ;
                      rdfs:domain voidPlus:MatchingMethod ;
                      rdfs:range voidPlus:MatchingAlgorithm ;
                      rdfs:comment "relates a voidPlus:MatchingMethod to its voidPlus:MatchingAlgorithm."@en .


###  http://lenticularlens.org/voidPlus/hasClassPartition
voidPlus:hasClassPartition rdf:type owl:ObjectProperty ;
                           rdfs:subPropertyOf voidPlus:hasSubset ,
                                              void:classPartition ;
                           rdfs:comment "relates a void:Dataset to its subset voidPlus:ClassPartition. In practice, the main difference wrt void:classPartition is the name meant to avoid miss-usage as it can be read as \"is classPartition of\" as well."@en .


###  http://lenticularlens.org/voidPlus/hasFormulation
voidPlus:hasFormulation rdf:type owl:ObjectProperty ;
                        rdfs:domain void:Dataset ;
                        rdfs:range voidPlus:Formulation ;
                        rdfs:comment "relates a voidPlus:Dataset to its voidPlus:Formulation."@en .


###  http://lenticularlens.org/voidPlus/hasItem
voidPlus:hasItem rdf:type owl:ObjectProperty ;
                 rdfs:domain voidPlus:Formulation ;
                 rdfs:comment "relates a voidPlus:Formulation to its formula-items."@en .


###  http://lenticularlens.org/voidPlus/hasLanguagePartition
voidPlus:hasLanguagePartition rdf:type owl:ObjectProperty ;
                              rdfs:subPropertyOf voidPlus:hasSubset ;
                              rdfs:comment "relates a void:Dataset to its subset voidPlus:LanguagePartition."@en .


###  http://lenticularlens.org/voidPlus/hasObjectResourceSelection
voidPlus:hasObjectResourceSelection rdf:type owl:ObjectProperty ;
                                    rdfs:subPropertyOf voidPlus:hasResourceSelection ;
                                    rdfs:comment "a relation to assign a voidPlus:ResourceSelection as the source for the objects of triples under scrutiny."@en .


###  http://lenticularlens.org/voidPlus/hasPropertyPartition
voidPlus:hasPropertyPartition rdf:type owl:ObjectProperty ;
                              rdfs:subPropertyOf voidPlus:hasSubset ,
                                                 void:propertyPartition ;
                              rdfs:comment "relates a void:Dataset to its subset voidPlus:PropertyPartition. In practice, the main difference wrt void:propertyPartition is the name meant to avoid miss-usage as it can be read as \"is propertyPartition of\" as well."@en .


###  http://lenticularlens.org/voidPlus/hasResourceSelection
voidPlus:hasResourceSelection rdf:type owl:ObjectProperty ;
                              rdfs:range voidPlus:ResourceSelection ;
                              rdfs:comment "a relation to assign a voidPlus:ResourceSelection as the source for entities under scrutiny.For example, the selection of a voidPlus:ResourceSelection for a voidPlus:MatchingMethod."@en .


###  http://lenticularlens.org/voidPlus/hasSubjectResourceSelection
voidPlus:hasSubjectResourceSelection rdf:type owl:ObjectProperty ;
                                     rdfs:subPropertyOf voidPlus:hasResourceSelection ;
                                     rdfs:comment "a relation to assign a voidPlus:ResourceSelection as the source for the subjects of triples under scrutiny."@en .


###  http://lenticularlens.org/voidPlus/hasSubset
voidPlus:hasSubset rdf:type owl:ObjectProperty ;
                   rdfs:subPropertyOf void:subset ;
                   owl:inverseOf voidPlus:subsetOf ;
                   rdfs:domain void:Dataset ;
                   rdfs:range voidPlus:Partition ;
                   rdfs:comment "relates a void:Dataset that has as subset a voidPlus:Partition (dataset). In practice, the main difference wrt void:subset is the name meant to avoid miss-usage as it can be read as \"is subset of\" as well. For a similar purpose, an inverse relation voidPlus:subsetOf is also defined."@en .


###  http://lenticularlens.org/voidPlus/hasTarget
voidPlus:hasTarget rdf:type owl:ObjectProperty ;
                   rdfs:domain voidPlus:LinkDataset ;
                   rdfs:range void:Dataset ;
                   rdfs:comment "A relation that assigns one or more void:Datasets linked via a voidPlus:LinkDataset."@en .


###  http://lenticularlens.org/voidPlus/hasValidation
voidPlus:hasValidation rdf:type owl:ObjectProperty ;
                       rdfs:domain voidPlus:LinkDataset ;
                       rdfs:range voidPlus:Validation ;
                       rdfs:comment "A relation that assigns one or more voidPlus:Validations to a voidPlus:LinkDataset."@en .


###  http://lenticularlens.org/voidPlus/language
voidPlus:language rdf:type owl:ObjectProperty ;
                  rdfs:subPropertyOf voidPlus:partitionedBy ;
                  rdfs:range voidPlus:Language ;
                  rdfs:comment "A relation that assigns to a void:Dataset a voidPlus:Language (for ISO standard language codes) that is the rdf:language of all literals (objects) qualifying entities (subject) in a language-based partition."@en .


###  http://lenticularlens.org/voidPlus/linkPredicate
voidPlus:linkPredicate rdf:type owl:ObjectProperty ;
                       rdfs:subPropertyOf owl:topObjectProperty ;
                       rdfs:comment "a link predicate that holds for a voidPlus:LinkDataset."@en .


###  http://lenticularlens.org/voidPlus/objectsTarget
voidPlus:objectsTarget rdf:type owl:ObjectProperty ;
                       rdfs:subPropertyOf voidPlus:hasTarget ;
                       rdfs:domain voidPlus:DirectedLinkDataset ;
                       rdfs:range void:Dataset ;
                       rdfs:comment "A relation that assigns void:Datasets describing the object of triples contained in the voidPlus:DirectedLinkDataset."@en .


###  http://lenticularlens.org/voidPlus/partitionedBy
voidPlus:partitionedBy rdf:type owl:ObjectProperty ;
                       rdfs:domain void:Dataset ;
                       rdfs:comment "A relation that assigns a void:Dataset to the conditions under which it is partitioned."@en .


###  http://lenticularlens.org/voidPlus/property
voidPlus:property rdf:type owl:ObjectProperty ;
                  rdfs:subPropertyOf voidPlus:partitionedBy ;
                  rdfs:range [ rdf:type owl:Class ;
                               owl:unionOf ( rdf:Property
                                             rdf:Seq
                                           )
                             ] ;
                  rdfs:comment "A relation that assigns to a void:Dataset a rdf:Property or a rdf:Seq of properties that expresses the pattern of all triples in a property-based partition."@en .


###  http://lenticularlens.org/voidPlus/subjectsTarget
voidPlus:subjectsTarget rdf:type owl:ObjectProperty ;
                        rdfs:subPropertyOf voidPlus:hasTarget ;
                        rdfs:domain voidPlus:DirectedLinkDataset ;
                        rdfs:range void:Dataset ;
                        rdfs:comment "A relation that assigns void:Datasets describing the subjects of triples contained in the voidPlus:DirectedLinkDataset."@en .


###  http://lenticularlens.org/voidPlus/subsetOf
voidPlus:subsetOf rdf:type owl:ObjectProperty ;
                  rdfs:comment "relates a voidPlus:Partition to its void:Dataset superset. Defined as the inverse relation of voidPlus:hasSubset."@en .


###  http://purl.org/dc/terms/creator
dcterms:creator rdf:type owl:ObjectProperty ;
                rdfs:comment "The range for dcterms:creator is dcterms:Agent. All values used with this property have to be instances of the class [dcterms:Agent] .  <span style=\"color: red\">must not be used with literal values</span>. You may use it only with non-literal values."@en .


###  http://purl.org/dc/terms/publisher
dcterms:publisher rdf:type owl:ObjectProperty ;
                  rdfs:range dcterms:Agent ;
                  rdfs:comment "The range for dcterms:publisher is dcterms:Agent. All values used with this property have to be instances of the class [dcterms:Agent] . <span style=\"color: red\">must not be used with literal values</span>. You may use it only with non-literal values."@en .


###  http://rdfs.org/ns/void#__linkPredicate
void:__linkPredicate rdf:type owl:ObjectProperty ;
                     rdfs:subPropertyOf voidPlus:linkPredicate ;
                     rdfs:domain void:Linkset ;
                     rdfs:range rdf:Property ;
                     rdfs:comment "a link predicate that holds for a void:Linkset."@en .


###  http://rdfs.org/ns/void#class
void:class rdf:type owl:ObjectProperty ;
           rdfs:subPropertyOf voidPlus:partitionedBy ;
           rdfs:range rdfs:Class ;
           rdfs:comment "A relation that assigns to a void:Dataset a rdfs:Class that is the rdf:type of all entities (subject) in a class-based partition."@en .


###  http://rdfs.org/ns/void#classPartition
void:classPartition rdf:type owl:ObjectProperty ;
                    rdfs:subPropertyOf void:subset ;
                    rdfs:comment "A relation between a void:Dataset and its Partition, which is a subset of a void:Dataset that contains only entities of an explicitly defined rdfs:Class."@en .


###  http://rdfs.org/ns/void#feature
void:feature rdf:type owl:ObjectProperty ;
             rdfs:domain void:Dataset ;
             rdfs:range void:TechnicalFeature ;
             rdfs:comment "relates a void:TechnicalFeature supported by a void:Datset."@en .


###  http://rdfs.org/ns/void#objectsTarget
void:objectsTarget rdf:type owl:ObjectProperty ;
                   rdfs:subPropertyOf voidPlus:objectsTarget ,
                                      void:target ;
                   rdfs:domain void:Linkset ;
                   rdfs:comment "A relation that assigns the void:Dataset describing the objects of triples contained in the void:Linkset."@en .


###  http://rdfs.org/ns/void#property
void:property rdf:type owl:ObjectProperty ;
              rdfs:subPropertyOf voidPlus:property ;
              rdfs:domain void:Dataset ;
              rdfs:range rdf:Property ;
              rdfs:comment "A relation that assigns to a void:Dataset a rdf:Property that is the predicate of all triples in a property-based partition."@en .


###  http://rdfs.org/ns/void#propertyPartition
void:propertyPartition rdf:type owl:ObjectProperty ;
                       rdfs:subPropertyOf void:subset ;
                       rdfs:comment "A relation between a void:Dataset and its Partition, which is a subset of a void:Dataset that contains  only triples composed with an explicitly defined rdf:Property."@en .


###  http://rdfs.org/ns/void#subjectsTarget
void:subjectsTarget rdf:type owl:ObjectProperty ;
                    rdfs:subPropertyOf voidPlus:subjectsTarget ,
                                       void:target ;
                    rdfs:domain void:Linkset ;
                    rdfs:comment "A relation that assigns the void:Dataset describing the subjects of triples contained in the void:Linkset."@en .


###  http://rdfs.org/ns/void#subset
void:subset rdf:type owl:ObjectProperty ;
            rdfs:domain void:Dataset ;
            rdfs:range void:Dataset ;
            rdfs:comment "relates a void:Dataset that has subset another void:Dataset."@en .


###  http://rdfs.org/ns/void#target
void:target rdf:type owl:ObjectProperty ;
            rdfs:subPropertyOf voidPlus:hasTarget ;
            rdfs:domain void:Linkset ;
            rdfs:range void:Dataset ;
            rdfs:comment "A relation that assigns one of the two void:Datasets linked by the void:Linkset."@en .


###  http://www.w3.org/2000/01/rdf-schema#member
rdfs:member rdf:type owl:ObjectProperty ;
            rdfs:comment "rdfs:member is an instance of rdf:Property that is a super-property of all the container membership properties. In particular, properties called rdf:_1, rdf:_2, rdf:_3... etc., used for rdf:Seq are sub-properties of rdfs:member."@en .


#################################################################
#    Data properties
#################################################################

###  http://creativecommons.org/ns#attributionName
<http://creativecommons.org/ns#attributionName> rdf:type owl:DatatypeProperty ;
                                                rdfs:comment "The name the creator of a Work would like used when attributing re-use."@en .


###  http://creativecommons.org/ns#license
<http://creativecommons.org/ns#license> rdf:type owl:DatatypeProperty ;
                                        rdfs:comment "A work has license a License."@en .


###  http://lenticularlens.org/voidPlus/hasAccepted
voidPlus:hasAccepted rdf:type owl:DatatypeProperty ;
                     rdfs:domain [ rdf:type owl:Class ;
                                   owl:unionOf ( voidPlus:LinkDataset
                                                 voidPlus:Validation
                                               )
                                 ] ;
                     rdfs:range xsd:integer ;
                     rdfs:comment "The amount of accepted links for a voidPlus:LinkDataset or voidPlus:Validation."@en .


###  http://lenticularlens.org/voidPlus/hasClusters
voidPlus:hasClusters rdf:type owl:DatatypeProperty ;
                     rdfs:domain voidPlus:LinkDataset ;
                     rdfs:range xsd:integer ;
                     rdfs:comment "The amount of clusters computed for a voidPlus:LinkDataset."@en .


###  http://lenticularlens.org/voidPlus/hasContradictions
voidPlus:hasContradictions rdf:type owl:DatatypeProperty ;
                           rdfs:domain voidPlus:LinkDataset ;
                           rdfs:range xsd:integer ;
                           rdfs:comment "The amount of links of a voidPlus:LinkDataset for which contradicting validations are found."@en .


###  http://lenticularlens.org/voidPlus/hasFilterFunction
voidPlus:hasFilterFunction rdf:type owl:DatatypeProperty ;
                           rdfs:domain voidPlus:PropertyPartition ;
                           rdfs:comment "It relates a property partition to a filter function, such as \"contains\" or \"minimal_date\". When restricting a property partition, in addition to the property for which a value is expected to exist, a filter can also be applied to the value. This filter is composed of \"function\", a \"value\" and a \"format\"."@en .


###  http://lenticularlens.org/voidPlus/hasFormatFunction
voidPlus:hasFormatFunction rdf:type owl:DatatypeProperty ;
                           rdfs:domain voidPlus:PropertyPartition ;
                           rdfs:comment "It relates a property partition to a format restriction which is applicable to the value used by an explicitly defined filter function, such as \"YYYY-MM-DD\" for filter \"minimal_date\". When restricting a property partition, in addition to the property for which a value is expected to exist, a filter can also be applied to the value. This filter is composed of \"function\", a \"value\" and a \"format\"."@en .


###  http://lenticularlens.org/voidPlus/hasFormulaDescription
voidPlus:hasFormulaDescription rdf:type owl:DatatypeProperty ;
                               rdfs:domain voidPlus:Formulation ;
                               rdfs:range xsd:string ;
                               rdfs:comment "Describes how items listed in a formulation are combined. For example, using logic or set-like operators."@en .


###  http://lenticularlens.org/voidPlus/hasRejected
voidPlus:hasRejected rdf:type owl:DatatypeProperty ;
                     rdfs:domain [ rdf:type owl:Class ;
                                   owl:unionOf ( voidPlus:LinkDataset
                                                 voidPlus:Validation
                                               )
                                 ] ;
                     rdfs:range xsd:integer ;
                     rdfs:comment "The amount of rejected links for a voidPlus:LinkDataset or voidPlus:Validation."@en .


###  http://lenticularlens.org/voidPlus/hasThreshold
voidPlus:hasThreshold rdf:type owl:DatatypeProperty ;
                      rdfs:domain voidPlus:MatchingMethod ;
                      rdfs:comment "Relates a voidPlus:MatchingMethod to a link-acceptance-threshold value. Upon the choice of a voidPlus:MatchingAlgorithm, the user should provide the parameters for guiding the acceptance of results. This may include a threshold value (e.g. 0,7 or 20), a threshold unit (e.g. \"Year\"), a threshold operator (e.g. \">=\") and a threshold range (e.g. \"]0,1]\" or \"ℕ\")."@en .


###  http://lenticularlens.org/voidPlus/hasThresholdAcceptanceOperator
voidPlus:hasThresholdAcceptanceOperator rdf:type owl:DatatypeProperty ;
                                        rdfs:domain voidPlus:MatchingMethod ;
                                        rdfs:comment "Relates a voidPlus:MatchingMethod to a link-acceptance-threshold operator. Upon the choice of a voidPlus:MatchingAlgorithm, the user should inform the parameters for guiding the acceptance of results. This may include a threshold value (e.g. 0,7 or 20), a threshold unit (e.g. \"Year\"), a threshold operator (e.g. \">=\") and a threshold range (e.g. \"]0,1]\" or \"ℕ\")."@en .


###  http://lenticularlens.org/voidPlus/hasThresholdRange
voidPlus:hasThresholdRange rdf:type owl:DatatypeProperty ;
                           rdfs:domain voidPlus:MatchingMethod ;
                           rdfs:comment "Relates a voidPlus:MatchingMethod to a link-acceptance-threshold range. Upon the choice of a voidPlus:MatchingAlgorithm, the user should inform the parameters for guiding the acceptance of results. This may include a threshold value (e.g. 0,7 or 20), a threshold unit (e.g. \"Year\"), a threshold operator (e.g. \">=\") and a threshold range (e.g. \"]0,1]\" or \"ℕ\")."@en .


###  http://lenticularlens.org/voidPlus/hasValidations
voidPlus:hasValidations rdf:type owl:DatatypeProperty ;
                        rdfs:domain [ rdf:type owl:Class ;
                                      owl:unionOf ( voidPlus:LinkDataset
                                                    voidPlus:Validation
                                                  )
                                    ] ;
                        rdfs:range xsd:integer ;
                        rdfs:comment "The amount of validated links in a voidPlus:LinkDataset or voidPlus:Validation."@en .


###  http://lenticularlens.org/voidPlus/hasValueFunction
voidPlus:hasValueFunction rdf:type owl:DatatypeProperty ;
                          rdfs:domain voidPlus:PropertyPartition ;
                          rdfs:comment "It relates a property partition to a value for a filter function, such as \"%van%\" for filter \"contains\" or \"01/01/1600\" for filter \"minimal_date\". When restricting a property partition, in addition to the property for which a value is expected to exist, a filter can also be applied to the value. This filter is composed of \"function\", a \"value\" and a \"format\"."@en .


###  http://lenticularlens.org/voidPlus/toBeValidated
voidPlus:toBeValidated rdf:type owl:DatatypeProperty ;
                       rdfs:domain [ rdf:type owl:Class ;
                                     owl:unionOf ( voidPlus:LinkDataset
                                                   voidPlus:Validation
                                                 )
                                   ] ;
                       rdfs:range xsd:integer ;
                       rdfs:comment "The amount of links yet to be validated in a voidPlus:LinkDataset or voidPlus:Validation."@en .


###  http://purl.org/dc/terms/created
dcterms:created rdf:type owl:DatatypeProperty ;
                rdfs:range rdfs:Literal ;
                rdfs:comment "The range defined for dcterms:created is the class of rdfs:Literal. Values used with this property therefore have to be literal values."@en .


###  http://purl.org/dc/terms/description
dcterms:description rdf:type owl:DatatypeProperty ;
                    rdfs:comment "There is no range defined for dcterms:description. Therefore you can use it with literal values."@en .


###  http://rdfs.org/ns/void#distinctObjects
void:distinctObjects rdf:type owl:DatatypeProperty ;
                     rdfs:domain void:Dataset ;
                     rdfs:range xsd:integer ;
                     rdfs:comment "The total number of distinct objects in a void:Dataset. In other words, the number of distinct resources that occur in the object position of triples in the dataset. Literals are included in this count." .


###  http://rdfs.org/ns/void#distinctSubjects
void:distinctSubjects rdf:type owl:DatatypeProperty ;
                      rdfs:domain void:Dataset ;
                      rdfs:range xsd:integer ;
                      rdfs:comment "The total number of distinct subjects in a void:Dataset. In other words, the number of distinct resources that occur in the subject position of triples in the dataset." .


###  http://rdfs.org/ns/void#entities
void:entities rdf:type owl:DatatypeProperty ;
              rdfs:domain void:Dataset ;
              rdfs:range xsd:integer ;
              rdfs:comment "The total number of entities that are described in a void:Dataset." .


###  http://rdfs.org/ns/void#triples
void:triples rdf:type owl:DatatypeProperty ;
             rdfs:domain void:Dataset ;
             rdfs:range xsd:integer ;
             rdfs:comment "The total number of triples contained in a void:Dataset."@en .


###  http://www.w3.org/2000/01/rdf-schema#label
rdfs:label rdf:type owl:DatatypeProperty .


#################################################################
#    Classes
#################################################################

###  http://lenticularlens.org/voidPlus/ClassPartition
voidPlus:ClassPartition rdf:type owl:Class ;
                        owl:equivalentClass [ rdf:type owl:Restriction ;
                                              owl:onProperty [ owl:inverseOf voidPlus:hasClassPartition
                                                             ] ;
                                              owl:someValuesFrom void:Dataset
                                            ] ,
                                            [ rdf:type owl:Restriction ;
                                              owl:onProperty void:class ;
                                              owl:qualifiedCardinality "1"^^xsd:nonNegativeInteger ;
                                              owl:onClass rdfs:Class
                                            ] ;
                        rdfs:subClassOf voidPlus:Partition ;
                        rdfs:comment "A voidPlus:Partition that is a collection of resources partitioned on the basis of an rdfs:Class."@en .


###  http://lenticularlens.org/voidPlus/DirectedLinkDataset
voidPlus:DirectedLinkDataset rdf:type owl:Class ;
                             owl:equivalentClass [ owl:intersectionOf ( [ rdf:type owl:Restriction ;
                                                                          owl:onProperty voidPlus:objectsTarget ;
                                                                          owl:someValuesFrom void:Dataset
                                                                        ]
                                                                        [ rdf:type owl:Restriction ;
                                                                          owl:onProperty voidPlus:subjectsTarget ;
                                                                          owl:someValuesFrom void:Dataset
                                                                        ]
                                                                      ) ;
                                                   rdf:type owl:Class
                                                 ] ;
                             rdfs:subClassOf voidPlus:LinkDataset ,
                                             [ rdf:type owl:Restriction ;
                                               owl:onProperty void:distinctObjects ;
                                               owl:qualifiedCardinality "1"^^xsd:nonNegativeInteger ;
                                               owl:onDataRange xsd:integer
                                             ] ,
                                             [ rdf:type owl:Restriction ;
                                               owl:onProperty void:distinctSubjects ;
                                               owl:qualifiedCardinality "1"^^xsd:nonNegativeInteger ;
                                               owl:onDataRange xsd:integer
                                             ] ;
                             rdfs:comment "A voidPlus:LinkDataset that imposes that subjects always belong to the same datasets as well as objects."@en .


###  http://lenticularlens.org/voidPlus/DocumentedLinkDataset
voidPlus:DocumentedLinkDataset rdf:type owl:Class ;
                               owl:equivalentClass [ owl:intersectionOf ( voidPlus:LinkDataset
                                                                          [ rdf:type owl:Restriction ;
                                                                            owl:onProperty voidPlus:hasFormulation ;
                                                                            owl:someValuesFrom voidPlus:Formulation
                                                                          ]
                                                                          [ rdf:type owl:Restriction ;
                                                                            owl:onProperty voidPlus:hasTarget ;
                                                                            owl:someValuesFrom voidPlus:ResourceSelection
                                                                          ]
                                                                          [ rdf:type owl:Restriction ;
                                                                            owl:onProperty voidPlus:hasTarget ;
                                                                            owl:allValuesFrom voidPlus:ResourceSelection
                                                                          ]
                                                                        ) ;
                                                     rdf:type owl:Class
                                                   ] ;
                               rdfs:subClassOf voidPlus:LinkDataset ;
                               rdfs:comment "A voidPlus:LinkDataset that requires detailed documentation, namely it imposes that targets are described as voidPlus:ResourceSelection and  requires a voidPlus:Formulation."@en .


###  http://lenticularlens.org/voidPlus/Formulation
voidPlus:Formulation rdf:type owl:Class ;
                     rdfs:comment "A (reusable) formulation that lists a number of items (e.g. matching methods or linksets) and describes how they are meant to be combined (e.g. using logic or set operators)."@en .


###  http://lenticularlens.org/voidPlus/IntegrationView
voidPlus:IntegrationView rdf:type owl:Class ;
                         rdfs:subClassOf void:Dataset ,
                                         [ owl:intersectionOf ( [ rdf:type owl:Restriction ;
                                                                  owl:onProperty voidPlus:hasSubset ;
                                                                  owl:minQualifiedCardinality "1"^^xsd:nonNegativeInteger ;
                                                                  owl:onClass voidPlus:LinkDataset
                                                                ]
                                                                [ rdf:type owl:Restriction ;
                                                                  owl:onProperty voidPlus:hasSubset ;
                                                                  owl:minQualifiedCardinality "2"^^xsd:nonNegativeInteger ;
                                                                  owl:onClass voidPlus:ResourceSelection
                                                                ]
                                                              ) ;
                                           rdf:type owl:Class
                                         ] ;
                         rdfs:comment "A set of RDF triples that are stemmed from two or more voidPlus:ResourceSelections that are linked by at least one voidPlus:LinkDataset. One may add voidPlus:PropertyPartitions for both filtering or for data visualisation and analysis."@en .


###  http://lenticularlens.org/voidPlus/Language
voidPlus:Language rdf:type owl:Class ;
                  rdfs:comment "A set of standardised language (ISO 639 not 3166) codes. For example, use nl, nld or dut to indicate the Dutch or Flemish languages."@en .


###  http://lenticularlens.org/voidPlus/LanguagePartition
voidPlus:LanguagePartition rdf:type owl:Class ;
                           owl:equivalentClass [ rdf:type owl:Restriction ;
                                                 owl:onProperty voidPlus:language ;
                                                 owl:someValuesFrom voidPlus:Language
                                               ] ,
                                               [ rdf:type owl:Restriction ;
                                                 owl:onProperty [ owl:inverseOf voidPlus:hasLanguagePartition
                                                                ] ;
                                                 owl:someValuesFrom void:Dataset
                                               ] ;
                           rdfs:subClassOf voidPlus:Partition ;
                           rdfs:comment "A voidPlus:Partition that is a collection of resources based on a voidPlus:Language restriction, i.e. an ISO 639 standardised language code."@en .


###  http://lenticularlens.org/voidPlus/Lens
voidPlus:Lens rdf:type owl:Class ;
              owl:equivalentClass [ owl:intersectionOf ( voidPlus:DocumentedLinkDataset
                                                         [ rdf:type owl:Restriction ;
                                                           owl:onProperty voidPlus:hasFormulation ;
                                                           owl:someValuesFrom voidPlus:LensFormulation
                                                         ]
                                                       ) ;
                                    rdf:type owl:Class
                                  ] ;
              rdfs:subClassOf voidPlus:DocumentedLinkDataset ;
              rdfs:comment "Similar to a voidPlus:Linkset (in the sense that it is a collection of links sharing the same linktype) also involving one, two or more datasets, but not necessarilly directed. Moreover, context-wise, it differs from a linkset as it is generated using different processes (set-like link manipulation operators such as Union, Intersection, Difference or Transitivity) as compared to how a linkset comes about (matching algorithms)."@en .


###  http://lenticularlens.org/voidPlus/LensFormulation
voidPlus:LensFormulation rdf:type owl:Class ;
                         rdfs:subClassOf voidPlus:Formulation ,
                                         [ rdf:type owl:Restriction ;
                                           owl:onProperty voidPlus:hasItem ;
                                           owl:minQualifiedCardinality "2"^^xsd:nonNegativeInteger ;
                                           owl:onClass voidPlus:LinkDataset
                                         ] ;
                         rdfs:comment "A resource that makes explicit all voidPlus:LinkDatasets involved in the creation of a voidPlus:Lens and how the they are combined."@en .


###  http://lenticularlens.org/voidPlus/LinkDataset
voidPlus:LinkDataset rdf:type owl:Class ;
                     owl:equivalentClass [ owl:intersectionOf ( [ rdf:type owl:Restriction ;
                                                                  owl:onProperty voidPlus:hasTarget ;
                                                                  owl:someValuesFrom void:Dataset
                                                                ]
                                                                [ rdf:type owl:Restriction ;
                                                                  owl:onProperty voidPlus:linkPredicate ;
                                                                  owl:someValuesFrom rdf:Property
                                                                ]
                                                              ) ;
                                           rdf:type owl:Class
                                         ] ;
                     rdfs:subClassOf void:Dataset ,
                                     [ rdf:type owl:Restriction ;
                                       owl:onProperty dcterms:description ;
                                       owl:someValuesFrom rdfs:Literal
                                     ] ;
                     rdfs:comment "A collection of RDF links between dataset(s), using the same link predicate (regardless of the link being an equality predicate or not). This predicate is called the linktype of the linkset. The links may have been stabilished among one (deduplication), two or many datasets."@en .


###  http://lenticularlens.org/voidPlus/Linkset
voidPlus:Linkset rdf:type owl:Class ;
                 owl:equivalentClass [ owl:intersectionOf ( voidPlus:DirectedLinkDataset
                                                            [ rdf:type owl:Restriction ;
                                                              owl:onProperty voidPlus:hasFormulation ;
                                                              owl:someValuesFrom voidPlus:LinksetFormulation
                                                            ]
                                                          ) ;
                                       rdf:type owl:Class
                                     ] ;
                 rdfs:subClassOf voidPlus:DirectedLinkDataset ,
                                 voidPlus:DocumentedLinkDataset ;
                 rdfs:comment "A collection of RDF links between <em>one</em>, <em>two</em> or  <em>more</em> void:Datasets. Only, all links share the same link-predicate and all subjects stem from a set of void datasets (D<sub>1</sub>) while all objects stem from either the same D<sub>1</sub> or a different set of void datasets D<sub>2</sub>."@en .


###  http://lenticularlens.org/voidPlus/LinksetFormulation
voidPlus:LinksetFormulation rdf:type owl:Class ;
                            rdfs:subClassOf voidPlus:Formulation ,
                                            [ rdf:type owl:Restriction ;
                                              owl:onProperty voidPlus:hasItem ;
                                              owl:someValuesFrom voidPlus:MatchingMethod
                                            ] ;
                            rdfs:comment "A resource that makes explicit all voidPlus:MatchingMethods involved in the creation of a voidPlus:Linkset and how the methods are logically joint."@en .


###  http://lenticularlens.org/voidPlus/MatchingAlgorithm
voidPlus:MatchingAlgorithm rdf:type owl:Class ;
                           rdfs:comment "A set of rules followed by a computer for finding pairs of matching resources. An algorithm can be further categorised as automated or semi-automated depending on whether it requires user assistance or not. Most matching algorithms employed in the Lenticular Lens are semi-automated."@en .


###  http://lenticularlens.org/voidPlus/MatchingMethod
voidPlus:MatchingMethod rdf:type owl:Class ;
                        owl:equivalentClass [ rdf:type owl:Restriction ;
                                              owl:onProperty voidPlus:hasAlgorithm ;
                                              owl:someValuesFrom voidPlus:MatchingAlgorithm
                                            ] ;
                        rdfs:comment "A resource that makes explicit all parameters/pre-requisites (datasets, entity-type and property-value restrictions, matching properties...) of a matching algorithm including the conditions in which the algorithm is to accept a discovered link (threshold)."@en .


###  http://lenticularlens.org/voidPlus/Partition
voidPlus:Partition rdf:type owl:Class ;
                   owl:equivalentClass [ rdf:type owl:Restriction ;
                                         owl:onProperty void:subset ;
                                         owl:someValuesFrom void:Dataset
                                       ] ;
                   rdfs:subClassOf void:Dataset ;
                   rdfs:comment "A void:Daset that is subset of another void:Daset."@en .


###  http://lenticularlens.org/voidPlus/PartitionFormulation
voidPlus:PartitionFormulation rdf:type owl:Class ;
                              rdfs:subClassOf voidPlus:Formulation ,
                                              [ rdf:type owl:Restriction ;
                                                owl:onProperty voidPlus:hasItem ;
                                                owl:someValuesFrom voidPlus:Partition
                                              ] .


###  http://lenticularlens.org/voidPlus/PropertyPartition
voidPlus:PropertyPartition rdf:type owl:Class ;
                           owl:equivalentClass [ rdf:type owl:Restriction ;
                                                 owl:onProperty [ owl:inverseOf voidPlus:hasPropertyPartition
                                                                ] ;
                                                 owl:someValuesFrom void:Dataset
                                               ] ,
                                               [ rdf:type owl:Restriction ;
                                                 owl:onProperty voidPlus:property ;
                                                 owl:qualifiedCardinality "1"^^xsd:nonNegativeInteger ;
                                                 owl:onClass [ rdf:type owl:Class ;
                                                               owl:unionOf ( rdf:Property
                                                                             rdf:Seq
                                                                           )
                                                             ]
                                               ] ;
                           rdfs:subClassOf voidPlus:Partition ;
                           rdfs:comment "A voidPlus:Partition that is is a collection of resources described using either a rdf:Property or sequence of them (voidPlus:PropertySequence or  voidPlus:TypedPropertySequence)."@en .


###  http://lenticularlens.org/voidPlus/PropertySequence
voidPlus:PropertySequence rdf:type owl:Class ;
                          owl:equivalentClass [ owl:intersectionOf ( [ rdf:type owl:Restriction ;
                                                                       owl:onProperty rdfs:member ;
                                                                       owl:allValuesFrom rdf:Property
                                                                     ]
                                                                     [ rdf:type owl:Restriction ;
                                                                       owl:onProperty rdfs:member ;
                                                                       owl:minQualifiedCardinality "2"^^xsd:nonNegativeInteger ;
                                                                       owl:onClass rdf:Property
                                                                     ]
                                                                   ) ;
                                                rdf:type owl:Class
                                              ] ;
                          rdfs:subClassOf rdf:Seq ;
                          rdfs:comment "A resource that represents a sequence of properties, analogously to a property path."@en .


###  http://lenticularlens.org/voidPlus/ResourceSelection
voidPlus:ResourceSelection rdf:type owl:Class ;
                           owl:equivalentClass [ owl:intersectionOf ( voidPlus:Partition
                                                                      [ rdf:type owl:Restriction ;
                                                                        owl:onProperty voidPlus:hasFormulation ;
                                                                        owl:someValuesFrom voidPlus:PartitionFormulation
                                                                      ]
                                                                    ) ;
                                                 rdf:type owl:Class
                                               ] ;
                           rdfs:subClassOf void:Dataset ,
                                           [ rdf:type owl:Restriction ;
                                             owl:onProperty voidPlus:hasSubset ;
                                             owl:someValuesFrom voidPlus:Partition
                                           ] ,
                                           [ rdf:type owl:Restriction ;
                                             owl:onProperty void:subset ;
                                             owl:someValuesFrom void:Dataset
                                           ] ,
                                           [ rdf:type owl:Restriction ;
                                             owl:onProperty dcterms:description ;
                                             owl:someValuesFrom rdfs:Literal
                                           ] ;
                           rdfs:comment "A collection of resources stemmed from the same void:Dataset. It is expected to have a voidPlus:ClassPartition as partition, directly or indirectly (i.e. as a subset). It can also have voidPlus:PropertyPartitions, where property-value(s) can be restricted, as well as voidPlus:LanguagePartitions, where the language of the property-value(s) can be restricted."@en .


###  http://lenticularlens.org/voidPlus/TypedPropertySequence
voidPlus:TypedPropertySequence rdf:type owl:Class ;
                               owl:equivalentClass [ owl:intersectionOf ( [ rdf:type owl:Restriction ;
                                                                            owl:onProperty rdfs:member ;
                                                                            owl:allValuesFrom [ rdf:type owl:Class ;
                                                                                                owl:unionOf ( rdf:Property
                                                                                                              rdfs:Class
                                                                                                            )
                                                                                              ]
                                                                          ]
                                                                          [ rdf:type owl:Restriction ;
                                                                            owl:onProperty rdfs:member ;
                                                                            owl:minQualifiedCardinality "1"^^xsd:nonNegativeInteger ;
                                                                            owl:onClass rdfs:Class
                                                                          ]
                                                                          [ rdf:type owl:Restriction ;
                                                                            owl:onProperty rdfs:member ;
                                                                            owl:minQualifiedCardinality "2"^^xsd:nonNegativeInteger ;
                                                                            owl:onClass rdf:Property
                                                                          ]
                                                                        ) ;
                                                     rdf:type owl:Class
                                                   ] ;
                               rdfs:subClassOf rdf:Seq ;
                               rdfs:comment """A resource that represents a sequence of properties and classes, as in a different type of property path with class restriction in between:
property -> class -> property -> class -> property"""@en .


###  http://lenticularlens.org/voidPlus/ValidatedLinkDataset
voidPlus:ValidatedLinkDataset rdf:type owl:Class ;
                              owl:equivalentClass [ owl:intersectionOf ( voidPlus:LinkDataset
                                                                         [ rdf:type owl:Restriction ;
                                                                           owl:onProperty voidPlus:hasValidation ;
                                                                           owl:someValuesFrom voidPlus:Validation
                                                                         ]
                                                                       ) ;
                                                    rdf:type owl:Class
                                                  ] ;
                              rdfs:subClassOf voidPlus:LinkDataset ,
                                              [ rdf:type owl:Restriction ;
                                                owl:onProperty voidPlus:hasContradictions ;
                                                owl:qualifiedCardinality "1"^^xsd:nonNegativeInteger ;
                                                owl:onDataRange xsd:integer
                                              ] ,
                                              [ rdf:type owl:Restriction ;
                                                owl:onProperty voidPlus:hasValidations ;
                                                owl:qualifiedCardinality "1"^^xsd:nonNegativeInteger ;
                                                owl:onDataRange xsd:integer
                                              ] ,
                                              [ rdf:type owl:Restriction ;
                                                owl:onProperty voidPlus:toBeValidated ;
                                                owl:qualifiedCardinality "1"^^xsd:nonNegativeInteger ;
                                                owl:onDataRange xsd:integer
                                              ] ;
                              rdfs:comment "A voidPlus:LinkDataset that has been validated."@en .


###  http://lenticularlens.org/voidPlus/Validation
voidPlus:Validation rdf:type owl:Class ;
                    owl:equivalentClass [ rdf:type owl:Restriction ;
                                          owl:onProperty [ owl:inverseOf voidPlus:hasValidation
                                                         ] ;
                                          owl:someValuesFrom voidPlus:LinkDataset
                                        ] ;
                    rdfs:subClassOf void:Dataset ,
                                    [ rdf:type owl:Restriction ;
                                      owl:onProperty voidPlus:hasAccepted ;
                                      owl:qualifiedCardinality "1"^^xsd:nonNegativeInteger ;
                                      owl:onDataRange xsd:integer
                                    ] ,
                                    [ rdf:type owl:Restriction ;
                                      owl:onProperty voidPlus:hasRejected ;
                                      owl:qualifiedCardinality "1"^^xsd:nonNegativeInteger ;
                                      owl:onDataRange xsd:integer
                                    ] ,
                                    [ rdf:type owl:Restriction ;
                                      owl:onProperty voidPlus:hasValidations ;
                                      owl:qualifiedCardinality "1"^^xsd:nonNegativeInteger ;
                                      owl:onDataRange xsd:integer
                                    ] ,
                                    [ rdf:type owl:Restriction ;
                                      owl:onProperty voidPlus:toBeValidated ;
                                      owl:qualifiedCardinality "1"^^xsd:nonNegativeInteger ;
                                      owl:onDataRange xsd:integer
                                    ] ;
                    rdfs:comment "A void:Dataset that contains triples describing the validaty of links stemmed from a voidPlus:LinkDataset."@en .


###  http://purl.org/dc/terms/Agent
dcterms:Agent rdf:type owl:Class ;
              rdfs:comment "A resource that acts or has the power to act."@en .


###  http://rdfs.org/ns/void#Dataset
void:Dataset rdf:type owl:Class ;
             rdfs:comment "A set of RDF triples that are published, maintained or aggregated by a single provider."@en .


###  http://rdfs.org/ns/void#Linkset
void:Linkset rdf:type owl:Class ;
             rdfs:subClassOf voidPlus:DirectedLinkDataset ,
                             [ owl:intersectionOf ( [ rdf:type owl:Restriction ;
                                                      owl:onProperty void:objectsTarget ;
                                                      owl:qualifiedCardinality "1"^^xsd:nonNegativeInteger ;
                                                      owl:onClass void:Dataset
                                                    ]
                                                    [ rdf:type owl:Restriction ;
                                                      owl:onProperty void:subjectsTarget ;
                                                      owl:qualifiedCardinality "1"^^xsd:nonNegativeInteger ;
                                                      owl:onClass void:Dataset
                                                    ]
                                                  ) ;
                               rdf:type owl:Class
                             ] ;
             rdfs:comment "A collection of RDF links between *two* void:Datasets."@en .


###  http://rdfs.org/ns/void#TechnicalFeature
void:TechnicalFeature rdf:type owl:Class ;
                      rdfs:comment "A technical feature of a void:Dataset, such as a supported RDF serialization format."@en .


###  http://www.w3.org/1999/02/22-rdf-syntax-ns#Property
rdf:Property rdf:type owl:Class ;
             rdfs:comment "The class of RDF properties."@en .


###  http://www.w3.org/1999/02/22-rdf-syntax-ns#Seq
rdf:Seq rdf:type owl:Class ;
        rdfs:comment "The class of RDF 'Sequence' containers."@en .


###  http://www.w3.org/2000/01/rdf-schema#Class
rdfs:Class rdf:type owl:Class ;
           rdfs:comment "This is the class of resources that are RDF classes."@en .


###  Generated by the OWL API (version 4.5.9.2019-02-01T07:24:44Z) https://github.com/owlcs/owlapi
